books/centaur/aig/aiger-help.lisp
@@ -36,46 +36,71 @@
 (include-book "std/basic/defs" :dir :system)
 (set-state-ok t)
 
+(local (in-theory (disable w)))
 
-(defun write-ascii-string1 (idx str stream state)
-  (declare (xargs :stobjs state
-                  :guard (and (symbolp stream)
+(defthm w-state-of-write-byte$
+  (equal (w (write-byte$ byte channel state))
+         (w state))
+  :hints(("Goal" :in-theory (enable write-byte$ w get-global))))
+
+(defthm w-state-of-read-byte$
+  (equal (w (mv-nth 1 (read-byte$ channel state)))
+         (w state))
+  :hints(("Goal" :in-theory (enable read-byte$ w get-global))))
+
+(define write-ascii-string1 (idx str stream state)
+  (declare (xargs :guard (and (symbolp stream)
                               (open-output-channel-p stream :byte state)
                               (stringp str)
                               (natp idx))
                   :measure (nfix (- (length str) (nfix idx)))))
+  :returns (new-state)
   (if (<= (length str) (lnfix idx))
       state
     (let ((state (write-byte$ (char-code (char str idx)) stream state)))
-      (write-ascii-string1 (1+ (lnfix idx)) str stream state))))
+      (write-ascii-string1 (1+ (lnfix idx)) str stream state)))
+  ///
+  (defret w-state-of-<fn>
+    (equal (w new-state) (w state)))
 
-(defthm open-output-channel-p1-of-write-ascii-string1
-  (implies (and (state-p1 state)
-                (symbolp stream)
-                (open-output-channel-p1 stream :byte state))
-           (let ((state (write-ascii-string1 idx str stream state)))
-             (and (state-p1 state)
-                  (open-output-channel-p1 stream :byte state)))))
+  (defthm open-output-channel-p1-of-write-ascii-string1
+    (implies (and (state-p1 state)
+                  (symbolp stream)
+                  (open-output-channel-p1 stream :byte state))
+             (let ((state (write-ascii-string1 idx str stream state)))
+               (and (state-p1 state)
+                    (open-output-channel-p1 stream :byte state))))))
 
-(defun write-ascii-string (str stream state)
-  (declare (xargs :stobjs state
-                  :guard (and (symbolp stream)
+(define write-ascii-string (str stream state)
+  (declare (xargs :guard (and (symbolp stream)
                               (open-output-channel-p stream :byte state)
                               (stringp str))))
-  (write-ascii-string1 0 str stream state))
+  :returns (new-state)
+  (write-ascii-string1 0 str stream state)
+  ///
+  (defret w-state-of-<fn>
+    (equal (w new-state) (w state)))
+
+  (defthm open-output-channel-p1-of-write-ascii-string
+    (implies (and (state-p1 state)
+                  (symbolp stream)
+                  (open-output-channel-p1 stream :byte state))
+             (let ((state (write-ascii-string str stream state)))
+               (and (state-p1 state)
+                    (open-output-channel-p1 stream :byte state))))))
 
 
 (encapsulate nil
   (local (include-book "ihs/quotient-remainder-lemmas" :dir :system))
   (local (in-theory (disable floor)))
-  (defun write-ascii-nat (n stream state)
-    (declare (xargs :stobjs state
-                    :guard (and (symbolp stream)
+  (define write-ascii-nat (n stream state)
+    (declare (xargs :guard (and (symbolp stream)
                                 (open-output-channel-p stream :byte state)
                                 (natp n))
                     :ruler-extenders :all
                     :measure (nfix n)
                     :verify-guards nil))
+    :returns (new-state)
     (b* ((n (lnfix n))
          (digit (mod n 10))
          (rest (floor n 10))
@@ -83,49 +108,52 @@
          (state (if (zp rest)
                     state
                   (write-ascii-nat rest stream state))))
-      (write-byte$ byte stream state)))
+      (write-byte$ byte stream state))
+    ///
+    (defthm open-output-channel-p1-of-write-ascii-nat
+      (implies (and (state-p1 state)
+                    (symbolp stream)
+                    (open-output-channel-p1 stream :byte state))
+               (let ((state (write-ascii-nat n stream state)))
+                 (and (state-p1 state)
+                      (open-output-channel-p1 stream :byte state)))))
 
-  (defthm open-output-channel-p1-of-write-ascii-nat
-    (implies (and (state-p1 state)
-                  (symbolp stream)
-                  (open-output-channel-p1 stream :byte state))
-             (let ((state (write-ascii-nat n stream state)))
-               (and (state-p1 state)
-                    (open-output-channel-p1 stream :byte state)))))
-
-  (verify-guards write-ascii-nat))
+    (verify-guards write-ascii-nat)
+    (defret w-state-of-<fn>
+      (equal (w new-state) (w state)))))
 
 
-(defund maybe-byte-p (x)
+(define maybe-byte-p (x)
   (declare (xargs :guard t))
   (or (not x)
-      (bytep x)))
+      (bytep x))
+  ///
 
-(defthm maybe-byte-p-of-byte
-  (implies (and (natp x) (< x 256))
-           (maybe-byte-p x))
-  :hints(("Goal" :in-theory (enable maybe-byte-p))))
+  (defthm maybe-byte-p-of-byte
+    (implies (and (natp x) (< x 256))
+             (maybe-byte-p x))
+    :hints(("Goal" :in-theory (enable maybe-byte-p))))
 
-(defthm maybe-byte-p-of-read-byte$
-  (implies (and (state-p1 state)
-                (symbolp stream)
-                (open-input-channel-p1 stream :byte state))
-           (maybe-byte-p (mv-nth 0 (read-byte$ stream state))))
-  :hints(("Goal" :in-theory (enable maybe-byte-p))))
+  (defthm maybe-byte-p-of-read-byte$
+    (implies (and (state-p1 state)
+                  (symbolp stream)
+                  (open-input-channel-p1 stream :byte state))
+             (maybe-byte-p (mv-nth 0 (read-byte$ stream state))))
+    :hints(("Goal" :in-theory (enable maybe-byte-p))))
 
-(defthm maybe-byte-p-compound-recognizer
-  (implies (maybe-byte-p x)
-           (or (not x)
-               (natp x)))
-  :hints(("Goal" :in-theory (enable maybe-byte-p)))
-  :rule-classes :compound-recognizer)
+  (defthm maybe-byte-p-compound-recognizer
+    (implies (maybe-byte-p x)
+             (or (not x)
+                 (natp x)))
+    :hints(("Goal" :in-theory (enable maybe-byte-p)))
+    :rule-classes :compound-recognizer)
 
-(defthm maybe-byte-p-bound
-  (implies (and (maybe-byte-p x)
-                x)
-           (< x 256))
-  :hints(("Goal" :in-theory (enable maybe-byte-p)))
-  :rule-classes :forward-chaining)
+  (defthm maybe-byte-p-bound
+    (implies (and (maybe-byte-p x)
+                  x)
+             (< x 256))
+    :hints(("Goal" :in-theory (enable maybe-byte-p)))
+    :rule-classes :forward-chaining))
 
 (local (defthm maybe-byte-p-bound-rw
          (implies (and (maybe-byte-p x) x)
@@ -133,11 +161,24 @@
          :rule-classes :rewrite))
 
 
+(define maybe-byte-fix ((x maybe-byte-p))
+  :inline t
+  :returns (new-x maybe-byte-p :rule-classes (:rewrite :type-prescription))
+  (mbe :logic (if (maybe-byte-p x) x 0)
+       :exec x)
+  ///
+  (defret maybe-byte-fix-when-maybe-byte-p
+    (implies (maybe-byte-p x)
+             (equal (maybe-byte-fix x) x))))
+  
 
 
-(defun-inline read-byte-buf (stream buf state)
-  (declare (xargs :stobjs state
-                  :guard (and (symbolp stream)
+
+
+(define read-byte-buf (stream buf state)
+  :inline t
+  :returns (mv byte new-buf new-state)
+  (declare (xargs :guard (and (symbolp stream)
                               (open-input-channel-p stream :byte state)
                               (maybe-byte-p buf))))
   (mbe :logic (mv-let (res buf state)
@@ -149,12 +190,13 @@
        :exec (if buf
                  (mv buf nil state)
                (b* (((mv byte state) (read-byte$ stream state)))
-                 (mv byte nil state)))))
+                 (mv byte nil state))))
+  ///
 
-(defthm maybe-byte-p-of-read-byte-buf-res
-  (maybe-byte-p (mv-nth 0 (read-byte-buf stream buf state)))
-  :rule-classes (:rewrite
-                 (:type-prescription
+  (defthm maybe-byte-p-of-read-byte-buf-res
+    (maybe-byte-p (mv-nth 0 (read-byte-buf stream buf state)))
+    :rule-classes (:rewrite
+                   (:type-prescription
 
 ; Added by Matt K., 8/9/2014: the :typed-term provided below was implicit
 ; before an ACL2 change considered for source function
@@ -167,16 +209,28 @@
 ; See also maybe-byte-p-of-peek-byte-buf-res, which has been modified in the
 ; same way for the same reason.
 
-                  :typed-term
-                  (mv-nth 0 (read-byte-buf stream buf state)))))
+                    :typed-term
+                    (mv-nth 0 (read-byte-buf stream buf state)))))
 
-(defthm maybe-byte-p-of-read-byte-buf-buf
-  (maybe-byte-p (mv-nth 1 (read-byte-buf stream buf state)))
-  :rule-classes (:rewrite :type-prescription))
+  (defthm maybe-byte-p-of-read-byte-buf-buf
+    (maybe-byte-p (mv-nth 1 (read-byte-buf stream buf state)))
+    :rule-classes (:rewrite :type-prescription))
+  
+  (defret w-state-of-<fn>
+    (equal (w new-state) (w state)))
 
-(defun-inline peek-byte-buf (stream buf state)
-  (declare (xargs :stobjs state
-                  :guard (and (symbolp stream)
+  (defthm open-input-channel-p1-of-read-byte-buf
+    (implies (and (symbolp stream)
+                  (state-p1 state)
+                  (open-input-channel-p1 stream :byte state))
+             (b* (((mv & & state) (read-byte-buf stream buf state)))
+               (and (open-input-channel-p1 stream :byte state)
+                    (state-p1 state))))))
+
+(define peek-byte-buf (stream buf state)
+  :inline t
+  :returns (mv byte new-buf new-state)
+  (declare (xargs :guard (and (symbolp stream)
                               (open-input-channel-p stream :byte state)
                               (maybe-byte-p buf))))
   (mbe :logic (mv-let (res buf state)
@@ -190,170 +244,176 @@
        :exec (if buf
                  (mv buf buf state)
                (b* (((mv byte state) (read-byte$ stream state)))
-                 (mv byte byte state)))))
+                 (mv byte byte state))))
+  ///
 
 
-(defthm maybe-byte-p-of-peek-byte-buf-res
-  (maybe-byte-p (mv-nth 0 (peek-byte-buf stream buf state)))
-  :rule-classes (:rewrite (:type-prescription
+  (defthm maybe-byte-p-of-peek-byte-buf-res
+    (maybe-byte-p (mv-nth 0 (peek-byte-buf stream buf state)))
+    :rule-classes (:rewrite (:type-prescription
 
 ; Added by Matt K., 8/9/2014: See the comment in
 ; maybe-byte-p-of-read-byte-buf-res, which is equally applicable here.
 
-                           :typed-term
-                           (mv-nth 0 (peek-byte-buf stream buf state)))))
+                             :typed-term
+                             (mv-nth 0 (peek-byte-buf stream buf state)))))
 
-(defthm maybe-byte-p-of-peek-byte-buf-buf
-  (maybe-byte-p (mv-nth 1 (peek-byte-buf stream buf state)))
-  :rule-classes (:rewrite :type-prescription))
+  (defthm maybe-byte-p-of-peek-byte-buf-buf
+    (maybe-byte-p (mv-nth 1 (peek-byte-buf stream buf state)))
+    :rule-classes (:rewrite :type-prescription))
 
-(defthm peek-byte-buf-of-peek-byte-buf
-  (implies (mv-nth 0 (peek-byte-buf stream buf state))
-           (equal (peek-byte-buf stream
-                                 (mv-nth 1 (peek-byte-buf stream buf state))
-                                 (mv-nth 2 (peek-byte-buf stream buf state)))
-                  (peek-byte-buf stream buf state))))
+  (defthm peek-byte-buf-of-peek-byte-buf
+    (implies (mv-nth 0 (peek-byte-buf stream buf state))
+             (equal (peek-byte-buf stream
+                                   (mv-nth 1 (peek-byte-buf stream buf state))
+                                   (mv-nth 2 (peek-byte-buf stream buf state)))
+                    (peek-byte-buf stream buf state))))
 
-(defun-inline skip-byte-buf (stream buf state)
+  (defthm open-input-channel-p1-of-peek-byte-buf
+    (implies (and (symbolp stream)
+                  (state-p1 state)
+                  (open-input-channel-p1 stream :byte state))
+             (b* (((mv & & state) (peek-byte-buf stream buf state)))
+               (and (open-input-channel-p1 stream :byte state)
+                    (state-p1 state)))))
+
+  (defret w-state-of-<fn>
+    (equal (w new-state) (w state))))
+
+(define skip-byte-buf (stream buf state)
+  :inline t
+  :returns (mv new-buf new-state)
   (declare (xargs :stobjs state
                   :guard (and (symbolp stream)
                               (open-input-channel-p stream :byte state))))
   (if buf
       (mv nil state)
     (b* (((mv & state) (read-byte$ stream state)))
-        (mv nil state))))
+      (mv nil state)))
+  ///
 
-(defthm maybe-byte-p-of-skip-byte-buf
-  (maybe-byte-p (mv-nth 0 (skip-byte-buf stream buf state)))
-  :rule-classes (:rewrite :type-prescription))
+  (defthm maybe-byte-p-of-skip-byte-buf
+    (maybe-byte-p (mv-nth 0 (skip-byte-buf stream buf state)))
+    :rule-classes (:rewrite :type-prescription))
 
-(defthm open-input-channel-p1-of-read-byte-buf
-  (implies (and (symbolp stream)
-                (state-p1 state)
-                (open-input-channel-p1 stream :byte state))
-           (b* (((mv & & state) (read-byte-buf stream buf state)))
-             (and (open-input-channel-p1 stream :byte state)
-                  (state-p1 state)))))
+  (defthm open-input-channel-p1-of-skip-byte-buf
+    (implies (and (symbolp stream)
+                  (state-p1 state)
+                  (open-input-channel-p1 stream :byte state))
+             (b* (((mv & state) (skip-byte-buf stream buf state)))
+               (and (open-input-channel-p1 stream :byte state)
+                    (state-p1 state)))))
 
-(defthm open-input-channel-p1-of-peek-byte-buf
-  (implies (and (symbolp stream)
-                (state-p1 state)
-                (open-input-channel-p1 stream :byte state))
-           (b* (((mv & & state) (peek-byte-buf stream buf state)))
-             (and (open-input-channel-p1 stream :byte state)
-                  (state-p1 state)))))
-
-(defthm open-input-channel-p1-of-skip-byte-buf
-  (implies (and (symbolp stream)
-                (state-p1 state)
-                (open-input-channel-p1 stream :byte state))
-           (b* (((mv & state) (skip-byte-buf stream buf state)))
-             (and (open-input-channel-p1 stream :byte state)
-                  (state-p1 state)))))
+  (defret w-state-of-<fn>
+    (equal (w new-state) (w state))))
 
 
 
-(defun aiger-buf-measure (stream buf state)
-  (declare (xargs :stobjs state
-                  :guard (and (symbolp stream)
+(define aiger-buf-measure (stream buf state)
+  (declare (xargs :guard (and (symbolp stream)
                               (open-input-channel-p stream :byte state)
                               (maybe-byte-p buf))))
-  (+ (if buf 1 0) (non-exec (file-measure stream state))))
+  (+ (if buf 1 0) (non-exec (file-measure stream state)))
+  ///
 
-(defthm aiger-buf-measure-of-read-byte-buf-weak
-  (b* (((mv & buf1 state1) (read-byte-buf stream buf state)))
-    (<= (aiger-buf-measure stream buf1 state1)
-        (aiger-buf-measure stream buf state)))
-  :rule-classes :linear)
+  (defthm aiger-buf-measure-of-read-byte-buf-weak
+    (b* (((mv & buf1 state1) (read-byte-buf stream buf state)))
+      (<= (aiger-buf-measure stream buf1 state1)
+          (aiger-buf-measure stream buf state)))
+    :hints(("Goal" :in-theory (enable read-byte-buf)))
+    :rule-classes :linear)
 
-(defthm aiger-buf-measure-of-read-byte-buf-strong
-  (b* (((mv res1 buf1 state1) (read-byte-buf stream buf state)))
-    (implies res1
-             (< (aiger-buf-measure stream buf1 state1)
-                (aiger-buf-measure stream buf state))))
-  :rule-classes :linear)
+  (defthm aiger-buf-measure-of-read-byte-buf-strong
+    (b* (((mv res1 buf1 state1) (read-byte-buf stream buf state)))
+      (implies res1
+               (< (aiger-buf-measure stream buf1 state1)
+                  (aiger-buf-measure stream buf state))))
+    :hints(("Goal" :in-theory (enable read-byte-buf)))
+    :rule-classes :linear)
 
-;; there is no strong
-(defthm aiger-buf-measure-of-peek-byte-buf
-  (b* (((mv & buf1 state1) (peek-byte-buf stream buf state)))
-    (<= (aiger-buf-measure stream buf1 state1)
-        (aiger-buf-measure stream buf state)))
-  :rule-classes :linear)
+  ;; there is no strong
+  (defthm aiger-buf-measure-of-peek-byte-buf
+    (b* (((mv & buf1 state1) (peek-byte-buf stream buf state)))
+      (<= (aiger-buf-measure stream buf1 state1)
+          (aiger-buf-measure stream buf state)))
+    :hints(("Goal" :in-theory (enable peek-byte-buf)))
+    :rule-classes :linear)
 
-;; there is no strong
-(defthm aiger-buf-measure-of-skip-byte-buf
-  (b* (((mv buf1 state1) (skip-byte-buf stream buf state)))
-    (<= (aiger-buf-measure stream buf1 state1)
-        (aiger-buf-measure stream buf state)))
-  :rule-classes :linear)
+  ;; there is no strong
+  (defthm aiger-buf-measure-of-skip-byte-buf
+    (b* (((mv buf1 state1) (skip-byte-buf stream buf state)))
+      (<= (aiger-buf-measure stream buf1 state1)
+          (aiger-buf-measure stream buf state)))
+    :hints(("Goal" :in-theory (enable skip-byte-buf)))
+    :rule-classes :linear)
 
-(defthm aiger-buf-measure-of-skip-byte-buf-strong-by-peek
-  (b* (((mv peek buf1 state1) (peek-byte-buf stream buf state))
-       ((mv buf2 state2) (skip-byte-buf stream buf1 state1)))
-    (implies peek
-             (< (aiger-buf-measure stream buf2 state2)
-                (aiger-buf-measure stream buf state))))
-  :rule-classes :linear)
-
-(in-theory (disable aiger-buf-measure
-                    read-byte-buf
-                    peek-byte-buf
-                    skip-byte-buf))
-
-
-
+  (defthm aiger-buf-measure-of-skip-byte-buf-strong-by-peek
+    (b* (((mv peek buf1 state1) (peek-byte-buf stream buf state))
+         ((mv buf2 state2) (skip-byte-buf stream buf1 state1)))
+      (implies peek
+               (< (aiger-buf-measure stream buf2 state2)
+                  (aiger-buf-measure stream buf state))))
+    :hints(("Goal" :in-theory (enable peek-byte-buf
+                                      skip-byte-buf)))
+    :rule-classes :linear))
 
 
-(defun read-ascii-nat1 (rest stream buf state)
-  (declare (xargs :stobjs state
-                  :guard (and (symbolp stream)
+
+
+
+(define read-ascii-nat1 (rest stream buf state)
+  (declare (xargs :guard (and (symbolp stream)
                               (open-input-channel-p stream :byte state)
                               (maybe-byte-p buf)
                               (natp rest))
                   :measure (aiger-buf-measure stream buf state)))
+  :returns (mv (nat natp :rule-classes :type-prescription)
+               (new-buf maybe-byte-p :rule-classes (:rewrite :type-prescription))
+               (new-state))
   (b* (((mv byte buf state) (peek-byte-buf stream buf state))
        ((when (not (and (integerp byte)
                         (<= (char-code #\0) byte)
                         (<= byte (char-code #\9)))))
-        (mv rest buf state))
+        (mv (lnfix rest) buf state))
        ((mv buf state) (skip-byte-buf stream buf state)))
     (read-ascii-nat1
-     (+ (* 10 rest) (- byte (char-code #\0)))
-     stream buf state)))
+     (+ (* 10 (lnfix rest)) (- byte (char-code #\0)))
+     stream buf state))
+  ///
 
-(defthm natp-read-ascii-nat1
-  (implies (natp rest)
-           (natp (mv-nth 0 (read-ascii-nat1 rest stream buf state))))
-  :hints(("Goal" :in-theory (enable read-ascii-nat1)))
-  :rule-classes (:rewrite :type-prescription))
+  (defthm open-input-channel-p1-of-read-ascii-nat1
+    (implies (and (state-p1 state)
+                  (symbolp stream)
+                  (open-input-channel-p1 stream :byte state))
+             (b* (((mv & & state)
+                   (read-ascii-nat1 rest stream buf state)))
+               (and (state-p1 state)
+                    (open-input-channel-p1 stream :byte state)))))
 
-(defthm open-input-channel-p1-of-read-ascii-nat1
-  (implies (and (state-p1 state)
-                (symbolp stream)
-                (open-input-channel-p1 stream :byte state))
-           (b* (((mv & & state)
-                 (read-ascii-nat1 rest stream buf state)))
-             (and (state-p1 state)
-                  (open-input-channel-p1 stream :byte state)))))
+  (defthm aiger-buf-measure-of-read-ascii-nat1
+    (b* (((mv & buf1 state1)
+          (read-ascii-nat1 rest stream buf state)))
+      (<= (aiger-buf-measure stream buf1 state1)
+          (aiger-buf-measure stream buf state)))
+    :rule-classes :linear)
 
-(defthm maybe-byte-p-of-read-ascii-nat1
-  (maybe-byte-p (mv-nth 1 (read-ascii-nat1 rest stream buf state)))
-  :rule-classes (:rewrite :type-prescription))
+  
+  (defret w-state-of-<fn>
+    (equal (w new-state) (w state))))
 
-(defthm aiger-buf-measure-of-read-ascii-nat1
-  (b* (((mv & buf1 state1)
-        (read-ascii-nat1 rest stream buf state)))
-    (<= (aiger-buf-measure stream buf1 state1)
-        (aiger-buf-measure stream buf state)))
-  :rule-classes :linear)
+(local (defthm maybe-natp-compound-recognzier
+         (equal (maybe-natp x)
+                (or (not x)
+                    (natp x)))
+         :rule-classes :compound-recognizer))
 
-(in-theory (disable read-ascii-nat1))
-
-(defun read-ascii-nat (stream buf state)
-  (declare (xargs :stobjs state
-                  :guard (and (symbolp stream)
+(define read-ascii-nat (stream buf state)
+  (declare (xargs :guard (and (symbolp stream)
                               (open-input-channel-p stream :byte state)
                               (maybe-byte-p buf))))
+  :returns (mv (res maybe-natp :rule-classes :type-prescription)
+               (new-buf maybe-byte-p :rule-classes (:rewrite :type-prescription))
+               (new-state))
   (b* (((mv byte buf state) (peek-byte-buf stream buf state))
        ((when (not (and (integerp byte)
                         (<= (char-code #\0) byte)
@@ -362,73 +422,66 @@
        ((mv buf state) (skip-byte-buf stream buf state)))
     (read-ascii-nat1
      (- byte (char-code #\0))
-     stream buf state)))
+     stream buf state))
+  ///
 
-(defthm natp-read-ascii-nat
-  (or (not (mv-nth 0 (read-ascii-nat stream buf state)))
-      (natp (mv-nth 0 (read-ascii-nat stream buf state))))
-  :hints(("Goal" :in-theory (enable read-ascii-nat)))
-  :rule-classes :type-prescription)
+  (defthm natp-read-ascii-nat-when-peek
+    (implies (b* ((n (mv-nth 0 (peek-byte-buf stream buf state))))
+               (and (integerp n)
+                    (<= (char-code #\0) n)
+                    (<= n (char-code #\9))))
+             (natp (mv-nth 0 (read-ascii-nat stream buf state))))
+    :hints(("Goal" :in-theory (enable read-ascii-nat))))
 
-(defthm natp-read-ascii-nat-when-peek
-  (implies (b* ((n (mv-nth 0 (peek-byte-buf stream buf state))))
-             (and (integerp n)
-                  (<= (char-code #\0) n)
-                  (<= n (char-code #\9))))
-           (natp (mv-nth 0 (read-ascii-nat stream buf state))))
-  :hints(("Goal" :in-theory (enable read-ascii-nat))))
+  (defthm integerp-read-ascii-nat-when-peek
+    ;; BOZO horrible
+    (implies (b* ((n (mv-nth 0 (peek-byte-buf stream buf state))))
+               (and (integerp n)
+                    (<= (char-code #\0) n)
+                    (<= n (char-code #\9))))
+             (integerp (mv-nth 0 (read-ascii-nat stream buf state))))
+    :hints(("Goal"
+            :in-theory (disable natp-read-ascii-nat-when-peek
+                                read-ascii-nat)
+            :use ((:instance natp-read-ascii-nat-when-peek)))))
 
-(defthm integerp-read-ascii-nat-when-peek
-  ;; BOZO horrible
-  (implies (b* ((n (mv-nth 0 (peek-byte-buf stream buf state))))
-             (and (integerp n)
-                  (<= (char-code #\0) n)
-                  (<= n (char-code #\9))))
-           (integerp (mv-nth 0 (read-ascii-nat stream buf state))))
-  :hints(("Goal"
-          :in-theory (disable natp-read-ascii-nat-when-peek
-                              read-ascii-nat)
-          :use ((:instance natp-read-ascii-nat-when-peek)))))
+  (defthm open-input-channel-p1-of-read-ascii-nat
+    (implies (and (state-p1 state)
+                  (symbolp stream)
+                  (open-input-channel-p1 stream :byte state))
+             (b* (((mv & & state)
+                   (read-ascii-nat stream buf state)))
+               (and (state-p1 state)
+                    (open-input-channel-p1 stream :byte state)))))
 
-(defthm open-input-channel-p1-of-read-ascii-nat
-  (implies (and (state-p1 state)
-                (symbolp stream)
-                (open-input-channel-p1 stream :byte state))
-           (b* (((mv & & state)
-                 (read-ascii-nat stream buf state)))
-             (and (state-p1 state)
-                  (open-input-channel-p1 stream :byte state)))))
+  (defthm aiger-buf-measure-of-read-ascii-nat-weak
+    (b* (((mv & buf1 state1)
+          (read-ascii-nat stream buf state)))
+      (<= (aiger-buf-measure stream buf1 state1)
+          (aiger-buf-measure stream buf state)))
+    :rule-classes :linear)
 
-(defthm maybe-byte-p-of-read-ascii-nat
-  (maybe-byte-p (mv-nth 1 (read-ascii-nat stream buf state))))
+  (defthm aiger-buf-measure-of-read-ascii-nat-strong
+    (b* (((mv res buf1 state1)
+          (read-ascii-nat stream buf state)))
+      (implies res
+               (< (aiger-buf-measure stream buf1 state1)
+                  (aiger-buf-measure stream buf state))))
+    :rule-classes :linear)
 
-(defthm aiger-buf-measure-of-read-ascii-nat-weak
-  (b* (((mv & buf1 state1)
-        (read-ascii-nat stream buf state)))
-    (<= (aiger-buf-measure stream buf1 state1)
-        (aiger-buf-measure stream buf state)))
-  :rule-classes :linear)
+  (defthm aiger-buf-measure-of-read-ascii-nat-strong1
+    (b* (((mv & buf1 state1)
+          (read-ascii-nat stream buf state))
+         (byte1 (mv-nth 0 (peek-byte-buf stream buf state))))
+      (implies (and (integerp byte1)
+                    (<= (char-code #\0) byte1)
+                    (<= byte1 (char-code #\9)))
+               (< (aiger-buf-measure stream buf1 state1)
+                  (aiger-buf-measure stream buf state))))
+    :rule-classes :linear)
 
-(defthm aiger-buf-measure-of-read-ascii-nat-strong
-  (b* (((mv res buf1 state1)
-        (read-ascii-nat stream buf state)))
-    (implies res
-             (< (aiger-buf-measure stream buf1 state1)
-                (aiger-buf-measure stream buf state))))
-  :rule-classes :linear)
-
-(defthm aiger-buf-measure-of-read-ascii-nat-strong1
-  (b* (((mv & buf1 state1)
-        (read-ascii-nat stream buf state))
-       (byte1 (mv-nth 0 (peek-byte-buf stream buf state))))
-    (implies (and (integerp byte1)
-                  (<= (char-code #\0) byte1)
-                  (<= byte1 (char-code #\9)))
-             (< (aiger-buf-measure stream buf1 state1)
-                (aiger-buf-measure stream buf state))))
-  :rule-classes :linear)
-
-(in-theory (disable read-ascii-nat))
+  (defret w-state-of-<fn>
+    (equal (w new-state) (w state))))
 
 
 
@@ -454,21 +507,6 @@
                  :induct t))
          :rule-classes :linear))
 
-(defun aiger-write-delta (n stream state)
-  (declare (xargs :guard (and (natp n)
-                              (symbolp stream)
-                              (open-output-channel-p stream :byte state))
-                  :verify-guards nil
-                  :measure (nfix n)
-                  :stobjs state))
-  (b* ((n (lnfix n))
-       (nextn (ash n -7))
-       (donep (zp nextn))
-       (newbyte (if donep n (logior #x80 (logand #x7F n))))
-       (state (write-byte$ newbyte stream state)))
-    (if donep
-        state
-      (aiger-write-delta nextn stream state))))
 
 (local
  (encapsulate nil
@@ -498,46 +536,69 @@
               :in-theory (disable unsigned-byte-p-of-logior
                                   unsigned-byte-p-of-loghead))))))
 
-(verify-guards aiger-write-delta)
+(define aiger-write-delta (n stream state)
+  (declare (xargs :guard (and (natp n)
+                              (symbolp stream)
+                              (open-output-channel-p stream :byte state))
+                  :verify-guards nil
+                  :measure (nfix n)))
+  :returns (new-state)
+  (b* ((n (lnfix n))
+       (nextn (ash n -7))
+       (donep (zp nextn))
+       (newbyte (if donep n (logior #x80 (logand #x7F n))))
+       (state (write-byte$ newbyte stream state)))
+    (if donep
+        state
+      (aiger-write-delta nextn stream state)))
+  ///
 
-(defthm open-output-channel-p1-of-aiger-write-delta
-  (implies (and (state-p1 state)
-                (symbolp stream)
-                (open-output-channel-p1 stream :byte state))
-           (let ((state (aiger-write-delta n stream state)))
-             (and (state-p1 state)
-                  (open-output-channel-p1 stream :byte state)))))
+  (defret w-state-of-<fn>
+    (equal (w new-state) (w state)))
 
 
-(defun write-char-separated-ascii-nat-list (lst sep stream state)
+  (verify-guards aiger-write-delta)
+
+  (defthm open-output-channel-p1-of-aiger-write-delta
+    (implies (and (state-p1 state)
+                  (symbolp stream)
+                  (open-output-channel-p1 stream :byte state))
+             (let ((state (aiger-write-delta n stream state)))
+               (and (state-p1 state)
+                    (open-output-channel-p1 stream :byte state))))))
+
+
+(define write-char-separated-ascii-nat-list (lst sep stream state)
   (declare (xargs :guard (and (symbolp stream)
                               (open-output-channel-p stream :byte state)
                               (nat-listp lst)
-                              (characterp sep))
-                  :stobjs state))
+                              (characterp sep))))
+  :returns (new-state)
   (if (atom lst)
       state
     (b* ((state (write-ascii-nat (car lst) stream state))
          (state (write-byte$ (char-code sep) stream state)))
       (write-char-separated-ascii-nat-list
-       (cdr lst) sep stream state))))
+       (cdr lst) sep stream state)))
+  ///
 
-(defthm open-output-channel-p1-of-write-char-separated-ascii-nat-list
-  (implies (and (state-p1 state)
-                (symbolp stream)
-                (open-output-channel-p1 stream :byte state))
-           (let ((state (write-char-separated-ascii-nat-list lst sep stream state)))
-             (and (state-p1 state)
-                  (open-output-channel-p1 stream :byte state)))))
+  (defret w-state-of-<fn>
+    (equal (w new-state) (w state)))
 
-(in-theory (disable write-char-separated-ascii-nat-list))
+  (defthm open-output-channel-p1-of-write-char-separated-ascii-nat-list
+    (implies (and (state-p1 state)
+                  (symbolp stream)
+                  (open-output-channel-p1 stream :byte state))
+             (let ((state (write-char-separated-ascii-nat-list lst sep stream state)))
+               (and (state-p1 state)
+                    (open-output-channel-p1 stream :byte state))))))
 
-(defun write-char-separated-ascii-nat-list-no-end (lst sep stream state)
+(define write-char-separated-ascii-nat-list-no-end (lst sep stream state)
   (declare (xargs :guard (and (symbolp stream)
                               (open-output-channel-p stream :byte state)
                               (nat-listp lst)
-                              (characterp sep))
-                  :stobjs state))
+                              (characterp sep))))
+  :returns (new-state)
   (if (atom lst)
       state
     (b* ((state (write-ascii-nat (car lst) stream state))
@@ -545,17 +606,19 @@
                     (write-byte$ (char-code sep) stream state)
                   state)))
       (write-char-separated-ascii-nat-list-no-end
-       (cdr lst) sep stream state))))
+       (cdr lst) sep stream state)))
+  ///
 
-(defthm open-output-channel-p1-of-write-char-separated-ascii-nat-list-no-end
-  (implies (and (state-p1 state)
-                (symbolp stream)
-                (open-output-channel-p1 stream :byte state))
-           (let ((state (write-char-separated-ascii-nat-list-no-end lst sep stream state)))
-             (and (state-p1 state)
-                  (open-output-channel-p1 stream :byte state)))))
+  (defret w-state-of-<fn>
+    (equal (w new-state) (w state)))
 
-(in-theory (disable write-char-separated-ascii-nat-list-no-end))
+  (defthm open-output-channel-p1-of-write-char-separated-ascii-nat-list-no-end
+    (implies (and (state-p1 state)
+                  (symbolp stream)
+                  (open-output-channel-p1 stream :byte state))
+             (let ((state (write-char-separated-ascii-nat-list-no-end lst sep stream state)))
+               (and (state-p1 state)
+                    (open-output-channel-p1 stream :byte state))))))
 
 
 (defun drop-trailing-0s (lst)
@@ -573,74 +636,81 @@
   (implies (nat-listp x)
            (nat-listp (drop-trailing-0s x))))
 
-(defun aiger-write-header (maxvar nins nlatches nouts ngates nbads ncnstrs stream state)
-  (declare (xargs :stobjs state
-                   :guard (and (symbolp stream)
-                               (open-output-channel-p stream :byte state)
-                               (natp maxvar) (natp nins) (natp nlatches) (natp nouts)
-                               (natp ngates) (natp nbads) (natp ncnstrs))))
+(define aiger-write-header (maxvar nins nlatches nouts ngates nbads ncnstrs stream state)
+  (declare (xargs :guard (and (symbolp stream)
+                              (open-output-channel-p stream :byte state)
+                              (natp maxvar) (natp nins) (natp nlatches) (natp nouts)
+                              (natp ngates) (natp nbads) (natp ncnstrs))))
+  :returns (new-state)
   (b* ((state (write-ascii-string "aig " stream state))
        (state (write-char-separated-ascii-nat-list-no-end
                (append (list maxvar nins nlatches nouts ngates)
                        (drop-trailing-0s (list nbads ncnstrs)))
                #\Space stream state))
        (state (write-byte$ (char-code #\Newline) stream state)))
-    state))
+    state)
+  ///
 
-(defthm open-output-channel-p1-of-aiger-write-header
-  (implies (and (state-p1 state)
-                (symbolp stream)
-                (open-output-channel-p1 stream :byte state))
-           (let ((state (aiger-write-header maxvar nins nlatches nouts ngates
-                                            nbads ncnstrs stream state)))
-             (and (state-p1 state)
-                  (open-output-channel-p1 stream :byte state)))))
+  (defret w-state-of-<fn>
+    (equal (w new-state) (w state)))
 
-(in-theory (disable aiger-write-header))
+  (defthm open-output-channel-p1-of-aiger-write-header
+    (implies (and (state-p1 state)
+                  (symbolp stream)
+                  (open-output-channel-p1 stream :byte state))
+             (let ((state (aiger-write-header maxvar nins nlatches nouts ngates
+                                              nbads ncnstrs stream state)))
+               (and (state-p1 state)
+                    (open-output-channel-p1 stream :byte state))))))
 
 
 
-(defun skip-ascii-chars (char stream buf state)
-  (declare (xargs :stobjs state
-                  :guard (and (symbolp stream)
+(define skip-ascii-chars (char stream buf state)
+  (declare (xargs :guard (and (symbolp stream)
                               (open-input-channel-p stream :byte state)
                               (characterp char)
                               (maybe-byte-p buf))
                   :measure (aiger-buf-measure stream buf state)))
+  :returns (mv (new-buf maybe-byte-p :rule-classes (:rewrite :type-prescription))
+               (new-state))
   (b* (((mv byte buf state) (peek-byte-buf stream buf state))
        ((when (not (eql byte (char-code char))))
         (mv buf state))
        ((mv buf state) (skip-byte-buf stream buf state)))
-    (skip-ascii-chars char stream buf state)))
+    (skip-ascii-chars char stream buf state))
+  ///
 
-(defthm open-input-channel-p1-of-skip-ascii-chars
-  (implies (and (state-p1 state)
-                (symbolp stream)
-                (open-input-channel-p1 stream :byte state))
-           (b* (((mv & state)
-                 (skip-ascii-chars char stream buf state)))
-             (and (state-p1 state)
-                  (open-input-channel-p1 stream :byte state)))))
+  (defthm open-input-channel-p1-of-skip-ascii-chars
+    (implies (and (state-p1 state)
+                  (symbolp stream)
+                  (open-input-channel-p1 stream :byte state))
+             (b* (((mv & state)
+                   (skip-ascii-chars char stream buf state)))
+               (and (state-p1 state)
+                    (open-input-channel-p1 stream :byte state)))))
 
-(defthm maybe-byte-p-of-skip-ascii-chars
-  (maybe-byte-p (mv-nth 0 (skip-ascii-chars char stream buf state)))
-  :rule-classes (:rewrite :type-prescription))
+  (defthm maybe-byte-p-of-skip-ascii-chars
+    (maybe-byte-p (mv-nth 0 (skip-ascii-chars char stream buf state)))
+    :rule-classes (:rewrite :type-prescription))
 
-(local (in-theory (disable skip-ascii-chars)))
+  (defret w-state-of-<fn>
+    (equal (w new-state) (w state))))
 
 
 
-(defun require-ascii-str1 (idx str stream buf state)
-  (declare (xargs :stobjs state
-                  :guard (and (symbolp stream)
+(define require-ascii-str1 (idx str stream buf state)
+  (declare (xargs :guard (and (symbolp stream)
                               (open-input-channel-p stream :byte state)
                               (natp idx)
                               (stringp str)
                               (<= idx (length str))
                               (maybe-byte-p buf))
                   :measure (nfix (- (length str) (nfix idx)))))
+  :returns (mv ok
+               (new-buf maybe-byte-p :rule-classes (:rewrite :type-prescription))
+               (new-state))
   (if (<= (length str) (lnfix idx))
-      (mv t buf state)
+      (mv t (maybe-byte-fix buf) state)
     (b* (((mv byte buf state)
           (peek-byte-buf stream buf state))
          ((when (or (not byte)
@@ -649,95 +719,108 @@
               (if byte (code-char byte) nil))
           (mv nil buf state))
          ((mv buf state) (skip-byte-buf stream buf state)))
-      (require-ascii-str1 (1+ (lnfix idx)) str stream buf state))))
+      (require-ascii-str1 (1+ (lnfix idx)) str stream buf state)))
+  ///
 
-(defthm open-input-channel-p1-of-require-ascii-str1
-  (implies (and (state-p1 state)
-                (symbolp stream)
-                (open-input-channel-p1 stream :byte state))
-           (b* (((mv & & state)
-                 (require-ascii-str1 idx str stream buf state)))
-             (and (state-p1 state)
-                  (open-input-channel-p1 stream :byte state)))))
+  (defthm open-input-channel-p1-of-require-ascii-str1
+    (implies (and (state-p1 state)
+                  (symbolp stream)
+                  (open-input-channel-p1 stream :byte state))
+             (b* (((mv & & state)
+                   (require-ascii-str1 idx str stream buf state)))
+               (and (state-p1 state)
+                    (open-input-channel-p1 stream :byte state)))))
 
-(defthm maybe-byte-p-of-require-ascii-str1
-  (implies (maybe-byte-p buf)
-           (maybe-byte-p (mv-nth 1 (require-ascii-str1 idx str stream buf
-                                                       statE))))
-  :rule-classes (:rewrite :type-prescription))
+  (defthm maybe-byte-p-of-require-ascii-str1
+    (implies (maybe-byte-p buf)
+             (maybe-byte-p (mv-nth 1 (require-ascii-str1 idx str stream buf
+                                                         statE))))
+    :rule-classes (:rewrite :type-prescription))
 
-(in-theory (disable  require-ascii-str1))
+  (defret w-state-of-<fn>
+    (equal (w new-state) (w state))))
 
-(defun require-ascii-str (str stream buf state)
-  (declare (xargs :stobjs state
-                  :guard (and (symbolp stream)
+(define require-ascii-str (str stream buf state)
+  (declare (xargs :guard (and (symbolp stream)
                               (open-input-channel-p stream :byte state)
                               (stringp str)
                               (maybe-byte-p buf))))
-  (require-ascii-str1 0 str stream buf state))
+  :returns (mv ok
+               (new-buf maybe-byte-p :rule-classes (:rewrite :type-prescription))
+               (new-state))
+  (require-ascii-str1 0 str stream buf state)
+  ///
 
-(defthm open-input-channel-p1-of-require-ascii-str
-  (implies (and (state-p1 state)
-                (symbolp stream)
-                (open-input-channel-p1 stream :byte state))
-           (b* (((mv & & state)
-                 (require-ascii-str str stream buf state)))
-             (and (state-p1 state)
-                  (open-input-channel-p1 stream :byte state)))))
+  (defthm open-input-channel-p1-of-require-ascii-str
+    (implies (and (state-p1 state)
+                  (symbolp stream)
+                  (open-input-channel-p1 stream :byte state))
+             (b* (((mv & & state)
+                   (require-ascii-str str stream buf state)))
+               (and (state-p1 state)
+                    (open-input-channel-p1 stream :byte state)))))
 
-(defthm maybe-byte-p-of-require-ascii-str
-  (implies (maybe-byte-p buf)
-           (maybe-byte-p (mv-nth 1 (require-ascii-str str stream buf statE))))
-  :rule-classes (:rewrite :type-prescription))
+  (defthm maybe-byte-p-of-require-ascii-str
+    (implies (maybe-byte-p buf)
+             (maybe-byte-p (mv-nth 1 (require-ascii-str str stream buf statE))))
+    :rule-classes (:rewrite :type-prescription))
 
-(in-theory (disable require-ascii-str))
+  (defret w-state-of-<fn>
+    (equal (w new-state) (w state))))
+
 
 
 
 ;; skips spaces and tabs
-(defun skip-linespace (stream buf state)
-  (declare (xargs :stobjs state
-                  :guard (and (symbolp stream)
+(define skip-linespace (stream buf state)
+  (declare (xargs :guard (and (symbolp stream)
                               (open-input-channel-p stream :byte state)
                               (maybe-byte-p buf))
                   :measure (aiger-buf-measure stream buf state)))
+  :returns (mv (new-buf maybe-byte-p :rule-classes (:rewrite :type-prescription))
+               (new-state))
   (b* (((mv byte buf state) (peek-byte-buf stream buf state))
        ((when (not (and (integerp byte)
                         (member (code-char byte) '(#\Space #\Tab)))))
         (mv buf state))
        ((mv buf state) (skip-byte-buf stream buf state)))
-    (skip-linespace stream buf state)))
+    (skip-linespace stream buf state))
+  ///
 
-(defthm open-input-channel-p1-of-skip-linespace
-  (implies (and (state-p1 state)
-                (symbolp stream)
-                (open-input-channel-p1 stream :byte state))
-           (b* (((mv & state)
-                 (skip-linespace stream buf state)))
-             (and (state-p1 state)
-                  (open-input-channel-p1 stream :byte state)))))
+  (defthm open-input-channel-p1-of-skip-linespace
+    (implies (and (state-p1 state)
+                  (symbolp stream)
+                  (open-input-channel-p1 stream :byte state))
+             (b* (((mv & state)
+                   (skip-linespace stream buf state)))
+               (and (state-p1 state)
+                    (open-input-channel-p1 stream :byte state)))))
 
-(defthm maybe-byte-p-of-skip-linespace
-  (maybe-byte-p (mv-nth 0 (skip-linespace stream buf state)))
-  :rule-classes (:rewrite :type-prescription))
+  (defthm maybe-byte-p-of-skip-linespace
+    (maybe-byte-p (mv-nth 0 (skip-linespace stream buf state)))
+    :rule-classes (:rewrite :type-prescription))
 
-(defthm aiger-buf-measure-of-skip-linespace
-  (b* (((mv  buf1 state1)
-        (skip-linespace stream buf state)))
-    (<= (aiger-buf-measure stream buf1 state1)
-        (aiger-buf-measure stream buf state)))
-  :rule-classes :linear)
+  (defthm aiger-buf-measure-of-skip-linespace
+    (b* (((mv  buf1 state1)
+          (skip-linespace stream buf state)))
+      (<= (aiger-buf-measure stream buf1 state1)
+          (aiger-buf-measure stream buf state)))
+    :rule-classes :linear)
 
-(in-theory (disable skip-linespace))
+  (defret w-state-of-<fn>
+    (equal (w new-state) (w state))))
 
 ;; Reads natural numbers until we come to some non-digit, non-space/tab
 ;; character.
-(defun read-nats-in-line (stream buf state)
+(define read-nats-in-line (stream buf state)
   (declare (xargs :stobjs state
                   :guard (and (symbolp stream)
                               (open-input-channel-p stream :byte state)
                               (maybe-byte-p buf))
                   :measure (aiger-buf-measure stream buf state)))
+  :returns (mv (nats nat-listp)
+               (new-buf maybe-byte-p :rule-classes (:rewrite :type-prescription))
+               (new-state))
   (b* (((mv buf state) (skip-linespace stream buf state))
        ((mv byte buf state) (peek-byte-buf stream buf state))
        ((unless (and (integerp byte)
@@ -746,56 +829,45 @@
         (mv nil buf state))
        ((mv head buf state) (read-ascii-nat stream buf state))
        ((mv rest buf state) (read-nats-in-line stream buf state)))
-    (mv (cons head rest) buf state)))
+    (mv (cons head rest) buf state))
+  ///
+  (defthm open-input-channel-p1-of-read-nats-in-line
+    (implies (and (state-p1 state)
+                  (symbolp stream)
+                  (open-input-channel-p1 stream :byte state))
+             (b* (((mv & & state)
+                   (read-nats-in-line stream buf state)))
+               (and (state-p1 state)
+                    (open-input-channel-p1 stream :byte state)))))
 
-(defthm open-input-channel-p1-of-read-nats-in-line
-  (implies (and (state-p1 state)
-                (symbolp stream)
-                (open-input-channel-p1 stream :byte state))
-           (b* (((mv & & state)
-                 (read-nats-in-line stream buf state)))
-             (and (state-p1 state)
-                  (open-input-channel-p1 stream :byte state)))))
+  (defthm aiger-buf-measure-of-read-nats-in-line
+    (b* (((mv & buf1 state1)
+          (read-nats-in-line stream buf state)))
+      (<= (aiger-buf-measure stream buf1 state1)
+          (aiger-buf-measure stream buf state)))
+    :rule-classes :linear)
 
-(defthm maybe-byte-p-of-read-nats-in-line
-  (maybe-byte-p (mv-nth 1 (read-nats-in-line stream buf state)))
-  :rule-classes (:rewrite :type-prescription))
+  (local (defthm integerp-when-natp
+           (implies (natp x)
+                    (integerp x))))
 
-(defthm maybe-byte-p-of-read-nats-in-line
-  (maybe-byte-p (mv-nth 1 (read-nats-in-line stream buf state)))
-  :rule-classes (:rewrite :type-prescription))
-
-(defthm aiger-buf-measure-of-read-nats-in-line
-  (b* (((mv & buf1 state1)
-        (read-nats-in-line stream buf state)))
-    (<= (aiger-buf-measure stream buf1 state1)
-        (aiger-buf-measure stream buf state)))
-  :rule-classes :linear)
-
-(local (defthm integerp-when-natp
-         (implies (natp x)
-                  (integerp x))))
-
-(defthm nat-listp-read-nats-in-line
-  (nat-listp (mv-nth 0 (read-nats-in-line stream buf state)))
-  :hints(("Goal" :in-theory (enable read-nats-in-line)))
-  :rule-classes
-  (:rewrite
-   (:forward-chaining :trigger-terms ((mv-nth 0 (read-nats-in-line stream buf state))))))
-
-(in-theory (disable read-nats-in-line))
+  (defret w-state-of-<fn>
+    (equal (w new-state) (w state))))
 
 (defun aiger-err (msg)
   (declare (xargs :guard t))
   msg)
 
-(defun read-bytecoded-nat (stream buf state)
-  (declare (xargs :stobjs state
-                  :guard (and (symbolp stream)
+(define read-bytecoded-nat (stream buf state)
+  (declare (xargs :guard (and (symbolp stream)
                               (open-input-channel-p stream :byte state)
                               (maybe-byte-p buf))
                   :verify-guards nil
                   :measure (aiger-buf-measure stream buf state)))
+  :returns (mv err
+               (val natp :rule-classes :type-prescription)
+               (new-buf maybe-byte-p :rule-classes (:rewrite :type-prescription))
+               (new-state))
   (b* (((mv byte buf state) (read-byte-buf stream buf state))
        ((when (not byte))
 
@@ -810,47 +882,40 @@
         (mv err 0 buf state)))
     (mv nil
         (+ (logand #x7F byte) (ash rest 7))
-        buf state)))
+        buf state))
+  ///
 
-(defthm natp-of-read-bytecoded-nat
-  (natp (mv-nth 1 (read-bytecoded-nat stream buf state)))
-  :rule-classes :type-prescription)
+  (verify-guards read-bytecoded-nat)
 
-(verify-guards read-bytecoded-nat)
+  (defthm open-input-channel-p1-of-read-bytecoded-nat
+    (implies (and (state-p1 state)
+                  (symbolp stream)
+                  (open-input-channel-p1 stream :byte state))
+             (b* (((mv & & & state)
+                   (read-bytecoded-nat stream buf state)))
+               (and (state-p1 state)
+                    (open-input-channel-p1 stream :byte state)))))
 
-(defthm open-input-channel-p1-of-read-bytecoded-nat
-  (implies (and (state-p1 state)
-                (symbolp stream)
-                (open-input-channel-p1 stream :byte state))
-           (b* (((mv & & & state)
-                 (read-bytecoded-nat stream buf state)))
-             (and (state-p1 state)
-                  (open-input-channel-p1 stream :byte state)))))
-
-(defthm maybe-byte-p-of-read-bytecoded-nat
-  (maybe-byte-p (mv-nth 2 (read-bytecoded-nat stream buf state)))
-  :rule-classes (:rewrite :type-prescription))
-
-
-(defthm aiger-buf-measure-of-read-bytecoded-nat-weak
-  (b* (((mv & & buf1 state1)
-        (read-bytecoded-nat stream buf state)))
-    (<= (aiger-buf-measure stream buf1 state1)
-        (aiger-buf-measure stream buf state)))
-  :hints (("goal" :induct (read-bytecoded-nat stream buf state)))
-  :rule-classes :linear)
+  (defthm aiger-buf-measure-of-read-bytecoded-nat-weak
+    (b* (((mv & & buf1 state1)
+          (read-bytecoded-nat stream buf state)))
+      (<= (aiger-buf-measure stream buf1 state1)
+          (aiger-buf-measure stream buf state)))
+    :hints (("goal" :induct (read-bytecoded-nat stream buf state)))
+    :rule-classes :linear)
 
 
-(defthm aiger-buf-measure-of-read-bytecoded-nat-strong
-  (b* (((mv err & buf1 state1)
-        (read-bytecoded-nat stream buf state)))
-    (implies (not err)
-             (< (aiger-buf-measure stream buf1 state1)
-                (aiger-buf-measure stream buf state))))
-  :hints (("goal" :induct (read-bytecoded-nat stream buf state)))
-  :rule-classes :linear)
+  (defthm aiger-buf-measure-of-read-bytecoded-nat-strong
+    (b* (((mv err & buf1 state1)
+          (read-bytecoded-nat stream buf state)))
+      (implies (not err)
+               (< (aiger-buf-measure stream buf1 state1)
+                  (aiger-buf-measure stream buf state))))
+    :hints (("goal" :induct (read-bytecoded-nat stream buf state)))
+    :rule-classes :linear)
 
-(in-theory (Disable read-bytecoded-nat))
+  (defret w-state-of-<fn>
+    (equal (w new-state) (w state))))
 
 
 
@@ -863,11 +928,19 @@
    :rule-classes (:rewrite :type-prescription)))
 
 
-(defun aiger-parse-header (stream buf state)
-  (declare (xargs :stobjs state
-                  :guard (and (symbolp stream)
+(define aiger-parse-header (stream buf state)
+  (declare (xargs :guard (and (symbolp stream)
                               (open-input-channel-p stream :byte state)
                               (maybe-byte-p buf))))
+  :returns (mv err
+               (n-ins natp :rule-classes :type-prescription)
+               (n-latches natp :rule-classes :type-prescription)
+               (n-ands natp :rule-classes :type-prescription)
+               (n-outs natp :rule-classes :type-prescription)
+               (n-bads natp :rule-classes :type-prescription)
+               (n-constrs natp :rule-classes :type-prescription)
+               (new-buf maybe-byte-p :rule-classes (:rewrite :type-prescription))
+               (new-state))
   (b* (((mv ok buf state) (require-ascii-str "aig" stream buf state))
        ((when (not ok))
         (mv (aiger-err "Bad header: no \"aig\"~%")
@@ -893,22 +966,17 @@
                      (equal f 0)))
         (mv (aiger-err "We don't support justice properties or fairness constraints yet~%")
             0 0 0 0 0 0 buf state)))
-    (mv nil i l a o b c buf state)))
+    (mv nil i l a o b c buf state))
+  ///
+  (defthm open-input-channel-p1-of-aiger-parse-header
+    (implies (and (state-p1 state)
+                  (symbolp stream)
+                  (open-input-channel-p1 stream :byte state))
+             (b* ((state
+                   (mv-nth 8 (aiger-parse-header stream buf state))))
+               (and (state-p1 state)
+                    (open-input-channel-p1 stream :byte state)))))
 
-(defthm open-input-channel-p1-of-aiger-parse-header
-  (implies (and (state-p1 state)
-                (symbolp stream)
-                (open-input-channel-p1 stream :byte state))
-           (b* ((state
-                 (mv-nth 8 (aiger-parse-header stream buf state))))
-             (and (state-p1 state)
-                  (open-input-channel-p1 stream :byte state)))))
+  (defret w-state-of-<fn>
+    (equal (w new-state) (w state))))
 
-(defthm maybe-byte-p-of-aiger-parse-header
-  (implies (maybe-byte-p buf)
-           (maybe-byte-p (mv-nth 7 (aiger-parse-header stream buf state))))
-  :rule-classes (:rewrite :type-prescription))
-
-(defmvtypes aiger-parse-header (nil natp natp natp natp natp natp nil nil))
-
-(in-theory (disable aiger-parse-header))
